examples/n_german/pad.thy
@@ -1,6 +1,6 @@
 (*proof(induct_tac e and f)
   fix x
-  show "?Pe (IVar x) s"
+  show "?Pe (IVar x) s"15210180295
   proof(case_tac "x")
     fix x1
     assume a1:"x=Ident x1"
@@ -574,3 +574,1029 @@ next
   show "?Pf (implyForm f1 f2) s"
     by(cut_tac a1 a2 ,auto)
 qed(auto)
+
+
+(*definition wellFormedParallel::"state\<Rightarrow>nat\<Rightarrow>nat\<Rightarrow>nat \<Rightarrow> statement list \<Rightarrow>bool " where [simp]:
+"wellFormedParallel s i M N SL\<equiv>  
+( \<forall>S'. S' \<in>set SL \<longrightarrow> 
+ ((\<exists>a. isBoundAssign s a i M  S') \<or> 
+  globalAssignment S' \<or>
+  (\<exists> f a SL'. S'=parallelList SL' \<and> wellDefinedForStatement s a N M f SL') ) )"
+
+
+definition wellFormedAndList11::"state\<Rightarrow>nat \<Rightarrow> nat\<Rightarrow>formula list\<Rightarrow>bool " where [simp]:
+"wellFormedAndList11 s N M fs\<equiv> (\<exists> fg. fs= (map (\<lambda>i. fg i) (down N)) \<and>
+( \<forall>i.  (isBoundFormula s i M (fg i)) ))"
+
+definition wellFormedAndList21::"state\<Rightarrow>nat \<Rightarrow> nat\<Rightarrow>nat\<Rightarrow>formula list\<Rightarrow>bool " where [simp]:
+"wellFormedAndList21 s N M i fs\<equiv> (\<exists> fg. fs=
+   (map (\<lambda>j. implyForm (neg (eqn (Const (index i)) (Const (index j)))) (fg j)) (down N)) \<and>
+( \<forall>i. (isBoundFormula s i M (fg i)) ))"
+
+definition wellFormedGuard::"state \<Rightarrow>nat \<Rightarrow> nat\<Rightarrow>nat \<Rightarrow>formula list\<Rightarrow>bool" where [simp]:
+"wellFormedGuard s N M i fs \<equiv>
+  ( (\<forall>g. g\<in>set fs \<longrightarrow>
+  (isBoundFormula s i M g \<or> 
+  (\<exists>gs. g=andList gs \<and>wellFormedAndList11 s  N M gs )\<or>
+  (\<exists>gs. g=andList gs \<and>wellFormedAndList21 s  N M i gs ) \<or> 
+  (\<exists>e1 e2. g=neg(eqn e1 e2)\<and>absTransfExp M e1=(Const (index (Suc M))) 
+  \<and>absTransfExp M e2=(Const (index (Suc M)))))))"
+
+primrec wellFormedGuardList::"state \<Rightarrow>nat \<Rightarrow> nat\<Rightarrow>nat \<Rightarrow>formula list\<Rightarrow>bool" where [simp]:
+"wellFormedGuardList s N M i [] = True"|
+"wellFormedGuardList s N M i (g#ls) = (wellFormedGuardList s N M i (ls)\<and>
+  (isBoundFormula s i M g \<or>
+  (\<exists>gs. g=andList gs \<and>wellFormedAndList11 s  N M gs )\<or>
+  (\<exists>gs. g=andList gs \<and>wellFormedAndList21 s  N M i gs ) \<or> 
+  (\<exists>e1 e2. g=neg(eqn e1 e2)\<and>absTransfExp M e1=(Const (index (Suc M))) 
+  \<and>absTransfExp M e2=(Const (index (Suc M)))))) "*)
+
+
+(*  by (smt absBoundExpFormLe absSafeExpFormGe absTransfForm.simps(8) b1 evalDontCareForm evalForall not_le)
+    using onWellAndList1 by blast*)
+  
+(*definition wellFormedGuard1::"state \<Rightarrow>nat \<Rightarrow> nat\<Rightarrow> nat \<Rightarrow>formula list\<Rightarrow>bool" where [simp]:
+"wellFormedGuard1 s N M i fs \<equiv>
+  ( (\<forall>g. g\<in>set fs \<longrightarrow>
+  (isBoundFormula s i M g \<or> wellFormedAndList1  N g 
+  \<or>wellFormedAndList2  N i g \<or> 
+  (\<exists>e1 e2. g=neg(eqn e1 e2)\<and>  ))))"*)
+
+(*lemma gloablAssign1:
+"globalAssignment  (assign as)\<longrightarrow>
+trans1 (boundIn M (assign as)) (abs1 M s) x =
+               absTransfConst M (expEval  (snd as) s) " *)
+
+(*proof(induct_tac S,simp)
+  fix as
+  show "?P (assign as)"
+  proof
+    assume a1:"isBoundAssign s a i M (assign as)"
+    have a2:" (  (fst as) =Para a i \<and> isBoundExp s i M (snd as)) "
+      by(cut_tac a1,auto)
+
+    then obtain a where a2:"(fst as) =Para a i \<and> isBoundExp s i M (snd as)"
+      by blast
+
+    show "abs1 M (trans1 (assign as) s) = trans1 (boundIn M (assign as)) (abs1 M s)"
+    proof
+      fix x
+      show "abs1 M (trans1 (assign as) s) x =
+         trans1 (boundIn M (assign as)) (abs1 M s) x "
+      proof(case_tac "(fst as \<noteq>x)")
+        assume b1:"fst as \<noteq> x"
+        show "abs1 M (trans1 (assign as) s) x =
+         trans1 (boundIn M (assign as)) (abs1 M s) x "
+          by(cut_tac b1,auto)
+      next
+        assume b1:"\<not> fst as \<noteq> x"
+        show "abs1 M (trans1 (assign as) s) x =
+         trans1 (boundIn M (assign as)) (abs1 M s) x "
+        proof(case_tac "i>M")
+          assume c1:"i>M"
+          show "abs1 M (trans1 (assign as) s) x =
+          trans1 (boundIn M (assign as)) (abs1 M s) x "
+            by(cut_tac c1 b1 a2,auto)
+        next  
+          assume c1:"~i>M"
+          have c2:"absTransfConst M (expEval (snd as) s)
+             =expEval (absTransfExp M (snd as)) (abs1 M s)"
+            using a2 absBoundExpForm assms c1 by fastforce 
+            
+          have c3:"abs1 M (trans1 (assign as) s) x=
+            absTransfConst M ((trans1 (assign as) s) x)"
+            apply(cut_tac a2 c1 b1,auto) 
+            done
+          show "abs1 M (trans1 (assign as) s) x =
+          trans1 (boundIn M (assign as)) (abs1 M s) x "
+            using a2 b1 c2 c3 by auto 
+        qed
+      qed
+    qed
+  qed
+qed(auto)
+*)
+  
+primrec varOfSents:: "statement list \<Rightarrow> varType set" where
+"varOfSents [] = {}"|
+"varOfSents (S#SL) = (varOfSent S) \<union> (varOfSents SL)"
+
+(*primrec mutualDiffDefinedStm::"statement \<Rightarrow> bool" where
+"mutualDiffDefinedStm skip =True" |
+"mutualDiffDefinedStm (assign as) =True"|
+"mutualDiffDefinedStm (parallel as P) = (mutualDiffDefinedStm P \<and> (fst as )\<notin>(varOfSent P))"*)
+
+primrec mutualDiffDefinedStmList::"statement list \<Rightarrow> bool" where
+"mutualDiffDefinedStmList [] =True" |
+"mutualDiffDefinedStmList (S#LS) =
+  (( (varOfSent S) \<inter>  (varOfSents  ( LS)) = {}) \<and>
+  ( mutualDiffDefinedStmList LS) \<and>
+   mutualDiffDefinedStm S)"
+
+lemma notAffect1:
+  shows "x \<notin>varOfSent S \<longrightarrow>trans1 (boundIn M S) s x =s x"
+  sorry
+
+lemma stateAbsAux1:
+  assumes a1:"mutualDiffDefinedStm S" and a2:"mutualDiffDefinedStmList (S # LS)"
+  and a3:"x \<in> varOfSent S"
+shows "mutualDiffDefinedStm S \<longrightarrow> 
+  mutualDiffDefinedStmList (S # LS)\<longrightarrow>
+  x \<in> varOfSent S \<longrightarrow>
+  abs1 M (trans1 (parallelList (S # LS)) s) x=
+  abs1 M (trans1 S  s) x" (is "?ant1 S \<longrightarrow> ?ant2 S\<longrightarrow>?ant3 S\<longrightarrow>?LHS S=?RHS S")
+  sorry
+(*proof(induct_tac S)
+  let ?S="skip" 
+  show "?ant1 ?S \<longrightarrow> ?ant2 ?S\<longrightarrow>?ant3 ?S\<longrightarrow>?LHS ?S=?RHS ?S"
+  proof(cut_tac  a3,auto)
+  qed
+next
+  fix x2
+  let ?S="assign x2"
+  
+  show "?ant1 ?S \<longrightarrow> ?ant2 ?S\<longrightarrow>?ant3 ?S\<longrightarrow>?LHS ?S=?RHS ?S"
+  proof(cut_tac  a3,auto)
+  qed
+next
+  fix x1 S
+  let  ?S = "parallel x1 S"
+  assume b0:"?ant1 S \<longrightarrow> ?ant2 S\<longrightarrow>?ant3 S\<longrightarrow>?LHS S=?RHS S"
+  show "?ant1 ?S \<longrightarrow> ?ant2 ?S\<longrightarrow>?ant3 ?S\<longrightarrow>?LHS ?S=?RHS ?S"
+  proof(rule impI)+
+    assume b1:"?ant1 ?S " and b2:"?ant2 ?S" and b3:"?ant3 ?S"
+    have c1:"fst x1=x |fst x1\<noteq>x" by blast
+    moreover
+    {assume c1:"fst x1=x"
+      have "?LHS ?S=?RHS ?S"
+      proof(cut_tac c1,auto)qed
+    }
+    moreover
+    {assume c1:"fst x1\<noteq>x"
+      have c2:"mutualDiffDefinedStm ( S)"
+        using b1 mutualDiffDefinedStm.simps(3) by blast
+      have c3:"?ant2 S"
+        apply(cut_tac b2,auto)done
+      have c4:"?ant3 S"
+        apply(cut_tac c1 b3,auto)done
+      have c5:"?LHS S=?RHS S"
+        using b0 c2 c3 c4 by blast 
+
+      have c6:"?LHS ?S=?LHS S"
+        using c1 parallelList.simps(2) by auto
+      have c7:"?RHS ?S=?RHS S"
+        using c1 by auto  
+        
+      have "?LHS ?S=?RHS ?S"
+        using c5 c6 c7 by auto
+         
+     
+    }
+    ultimately show "?LHS ?S=?RHS ?S"
+      by blast
+  qed
+qed
+*)  
+lemma stateAbsAux2:
+  assumes a1:"mutualDiffDefinedStm S" and a2:"mutualDiffDefinedStmList (S # LS)"
+  and a3:"x \<in> varOfSent S"
+shows "mutualDiffDefinedStm S \<longrightarrow> 
+  mutualDiffDefinedStmList (S # LS)\<longrightarrow>
+  x \<in> varOfSent S \<longrightarrow>trans1 (boundIn M (parallelList (S # LS))) (abs1 M s) x=
+        trans1 (boundIn M (  (S ))) (abs1 M s) x"
+(is "?ant1 S \<longrightarrow> ?ant2 S\<longrightarrow>?ant3 S\<longrightarrow>?LHS S=?RHS S")
+(*proof(induct_tac S)
+  let ?S="skip" 
+  show "?ant1 ?S \<longrightarrow> ?ant2 ?S\<longrightarrow>?ant3 ?S\<longrightarrow>?LHS ?S=?RHS ?S"
+  proof(cut_tac  a3,auto)
+  qed
+next
+  fix x2
+  let ?S="assign x2"
+  
+  show "?ant1 ?S \<longrightarrow> ?ant2 ?S\<longrightarrow>?ant3 ?S\<longrightarrow>?LHS ?S=?RHS ?S"
+  proof(case_tac "fst x2",cut_tac  a3,force)
+    fix x21 x22
+    assume b1:"fst x2 = Para x21 x22"
+    show "?ant1 ?S \<longrightarrow> ?ant2 ?S\<longrightarrow>?ant3 ?S\<longrightarrow>?LHS ?S=?RHS ?S"
+      apply(cut_tac b1,simp)
+      apply(subgoal_tac "x \<notin>varOfSent (parallelList LS)")
+      using notAffect1 apply auto[1] 
+      sorry
+  next
+    assume b1:"fst x2=dontCareVar"
+    show "?ant1 ?S \<longrightarrow> ?ant2 ?S\<longrightarrow>?ant3 ?S\<longrightarrow>?LHS ?S=?RHS ?S"
+      apply(cut_tac b1,simp)
+      apply(subgoal_tac "x \<notin>varOfSent (parallelList LS)")
+      using notAffect1 apply auto[1] 
+      sorry
+  qed
+next
+  fix x1 S
+  let  ?S = "parallel x1 S"
+  assume b0:"?ant1 S \<longrightarrow> ?ant2 S\<longrightarrow>?ant3 S\<longrightarrow>?LHS S=?RHS S"
+  show "?ant1 ?S \<longrightarrow> ?ant2 ?S\<longrightarrow>?ant3 ?S\<longrightarrow>?LHS ?S=?RHS ?S"
+  proof(rule impI)+
+    assume b1:"?ant1 ?S " and b2:"?ant2 ?S" and b3:"?ant3 ?S"
+    have c1:"fst x1=x |fst x1\<noteq>x" by blast
+    moreover
+    {assume c1:"fst x1=x"
+      have c2:"x \<notin> varOfSent S"
+        using b1 c1 mutualDiffDefinedStm.simps(3) by blast 
+      have c2:"x \<notin> varOfSent (cat S (parallelList LS))"
+        sorry
+      have "?LHS ?S=?RHS ?S"
+        apply(cut_tac c1,case_tac "fst x1",force)
+         apply(case_tac "x22>M",auto)
+        using c2 notAffect1 apply auto[1]
+        using c2 notAffect1 by auto 
+    }
+    moreover
+    {assume c1:"fst x1\<noteq>x"
+      have c2:"mutualDiffDefinedStm ( S)"
+        using b1 mutualDiffDefinedStm.simps(3) by blast
+      have c3:"?ant2 S"
+        apply(cut_tac b2,auto)done
+      have c4:"?ant3 S"
+        apply(cut_tac c1 b3,auto)done
+      have c5:"?LHS S=?RHS S"
+        using b0 c2 c3 c4 by blast 
+
+      have c6:"?LHS ?S=?LHS S"
+        using c1 parallelList.simps(2) by auto
+      have c7:"?RHS ?S=?RHS S"
+        using c1 by auto  
+        
+      have "?LHS ?S=?RHS ?S"
+        using c5 c6 c7 by auto
+         
+     
+    }
+    ultimately show "?LHS ?S=?RHS ?S"
+      by blast
+  qed
+qed
+*)
+sorry
+lemma stateAbsAux3:
+  assumes a1:"mutualDiffDefinedStm S" and a2:"mutualDiffDefinedStmList (S # LS)"
+  and a3:"x \<notin> varOfSent S"
+shows "mutualDiffDefinedStm S \<longrightarrow> 
+  mutualDiffDefinedStmList (S # LS)\<longrightarrow>
+  x \<notin> varOfSent S \<longrightarrow>abs1 M (trans1 (parallelList (S # LS)) s) x=
+      abs1 M (trans1 (parallelList (  LS))  s) x"
+(is "?ant1 S \<longrightarrow> ?ant2 S\<longrightarrow>?ant3 S\<longrightarrow>?LHS S=?RHS S")
+sorry
+(*proof(induct_tac S)
+  let ?S="skip" 
+  show "?ant1 ?S \<longrightarrow> ?ant2 ?S\<longrightarrow>?ant3 ?S\<longrightarrow>?LHS ?S=?RHS ?S"
+  proof(cut_tac  a3,auto)
+  qed
+next
+  fix x2
+  let ?S="assign x2"
+  
+  show "?ant1 ?S \<longrightarrow> ?ant2 ?S\<longrightarrow>?ant3 ?S\<longrightarrow>?LHS ?S=?RHS ?S"
+  proof(case_tac "fst x2",cut_tac  a3,force)
+    fix x21 x22
+    assume b1:"fst x2 = Para x21 x22"
+    show "?ant1 ?S \<longrightarrow> ?ant2 ?S\<longrightarrow>?ant3 ?S\<longrightarrow>?LHS ?S=?RHS ?S"
+      apply(cut_tac b1,simp)
+      by blast
+       
+  next
+    assume b1:"fst x2=dontCareVar"
+    show "?ant1 ?S \<longrightarrow> ?ant2 ?S\<longrightarrow>?ant3 ?S\<longrightarrow>?LHS ?S=?RHS ?S"
+      apply(cut_tac b1,simp)
+      by blast
+      
+  qed
+next
+  fix x1 S
+  let  ?S = "parallel x1 S"
+  assume b0:"?ant1 S \<longrightarrow> ?ant2 S\<longrightarrow>?ant3 S\<longrightarrow>?LHS S=?RHS S"
+  show "?ant1 ?S \<longrightarrow> ?ant2 ?S\<longrightarrow>?ant3 ?S\<longrightarrow>?LHS ?S=?RHS ?S"
+  proof(rule impI)+
+    assume b1:"?ant1 ?S " and b2:"?ant2 ?S" and b3:"?ant3 ?S"
+    have c1:"fst x1=x |fst x1\<noteq>x" by blast
+    moreover
+    {assume c1:"fst x1=x"
+      have c2:"False"
+        using b3 c1 by auto
+       
+      have "?LHS ?S=?RHS ?S"
+        
+        using c2 notAffect1 by auto 
+    }
+    moreover
+    {assume c1:"fst x1\<noteq>x"
+      have c2:"mutualDiffDefinedStm ( S)"
+        using b1 mutualDiffDefinedStm.simps(3) by blast
+      have c3:"?ant2 S"
+        apply(cut_tac b2,auto)done
+      have c4:"?ant3 S"
+        apply(cut_tac c1 b3,auto)done
+      have c5:"?LHS S=?RHS S"
+        using b0 c2 c3 c4 by blast 
+
+      have c6:"?LHS ?S=?LHS S"
+        using c1 parallelList.simps(2) by auto
+      have c7:"?RHS ?S=?RHS S"
+        using c1 by auto  
+        
+      have "?LHS ?S=?RHS ?S"
+        using c5 c6 c7 by auto
+         
+     
+    }
+    ultimately show "?LHS ?S=?RHS ?S"
+      by blast
+  qed
+qed
+*)
+   
+ 
+lemma stateAbsAux4:
+  assumes a1:"mutualDiffDefinedStm S" and a2:"mutualDiffDefinedStmList (S # LS)"
+  and a3:"x \<notin> varOfSent S"
+shows "mutualDiffDefinedStm S \<longrightarrow> 
+  mutualDiffDefinedStmList (S # LS)\<longrightarrow>
+  x \<notin> varOfSent S \<longrightarrow>trans1 (boundIn M (parallelList (S # LS))) (abs1 M s) x=
+        trans1 (boundIn M (parallelList  LS)) (abs1 M s) x"
+
+(is "?ant1 S \<longrightarrow> ?ant2 S\<longrightarrow>?ant3 S\<longrightarrow>?LHS S=?RHS S")
+  sorry
+(*proof(induct_tac S)
+  let ?S="skip" 
+  show "?ant1 ?S \<longrightarrow> ?ant2 ?S\<longrightarrow>?ant3 ?S\<longrightarrow>?LHS ?S=?RHS ?S"
+  proof(cut_tac  a3,auto)
+  qed
+next
+  fix x2
+  let ?S="assign x2"
+  
+  show "?ant1 ?S \<longrightarrow> ?ant2 ?S\<longrightarrow>?ant3 ?S\<longrightarrow>?LHS ?S=?RHS ?S"
+  proof(case_tac "fst x2",cut_tac  a3,force)
+    fix x21 x22
+    assume b1:"fst x2 = Para x21 x22"
+    show "?ant1 ?S \<longrightarrow> ?ant2 ?S\<longrightarrow>?ant3 ?S\<longrightarrow>?LHS ?S=?RHS ?S"
+      apply(cut_tac b1,simp)
+      done
+       
+  next
+    assume b1:"fst x2=dontCareVar"
+    show "?ant1 ?S \<longrightarrow> ?ant2 ?S\<longrightarrow>?ant3 ?S\<longrightarrow>?LHS ?S=?RHS ?S"
+      apply(cut_tac b1,simp)
+     done
+      
+  qed
+next
+  fix x1 S
+  let  ?S = "parallel x1 S"
+  assume b0:"?ant1 S \<longrightarrow> ?ant2 S\<longrightarrow>?ant3 S\<longrightarrow>?LHS S=?RHS S"
+  show "?ant1 ?S \<longrightarrow> ?ant2 ?S\<longrightarrow>?ant3 ?S\<longrightarrow>?LHS ?S=?RHS ?S"
+  proof(rule impI)+
+    assume b1:"?ant1 ?S " and b2:"?ant2 ?S" and b3:"?ant3 ?S"
+    have c1:"fst x1=x |fst x1\<noteq>x" by blast
+    moreover
+    {assume c1:"fst x1=x"
+      have c2:"False"
+        using b3 c1 by auto
+       
+      have "?LHS ?S=?RHS ?S"
+        
+        using c2 notAffect1 by auto 
+    }
+    moreover
+    {assume c1:"fst x1\<noteq>x"
+      have c2:"mutualDiffDefinedStm ( S)"
+        using b1 mutualDiffDefinedStm.simps(3) by blast
+      have c3:"?ant2 S"
+        apply(cut_tac b2,auto)done
+      have c4:"?ant3 S"
+        apply(cut_tac c1 b3,auto)done
+      have c5:"?LHS S=?RHS S"
+        using b0 c2 c3 c4 by blast 
+
+      have c6:"?LHS ?S=?LHS S"
+        using c1 parallelList.simps(2) by auto
+      have c7:"?RHS ?S=?RHS S"
+        using c1 by auto  
+        
+      have "?LHS ?S=?RHS ?S"
+        using c5 c6 c7 by auto
+         
+     
+    }
+    ultimately show "?LHS ?S=?RHS ?S"
+      by blast
+  qed
+qed
+*)s
+
+boundIn M skip =skip"|
+"boundIn M (assign as) = 
+  (if absTransfVar M (fst as) = dontCareVar 
+  then skip else (assign  ((fst as), (absTransfExp M (snd as)))))" |
+"boundIn M (parallel as S) =
+   parallel  (boundIn M as) (boundIn M S)" |
+"boundIn M (forallStm PS N) =
+   forallStm (\<lambda>i. boundIn M (PS i)) M" 
+
+lemma absStmIsSkip:
+  assumes a1:"s dontCareVar =dontCare"
+  shows "(absTransfStatement M S) =skip\<longrightarrow>
+ abs1 M (trans1 S s) = trans1 (absTransfStatement M S) (abs1 M s)"
+(is "?P S") \<Rightarrow> nat
+  sorry
+(*
+proof(induct_tac S)
+  let ?S="skip"
+  show "?P ?S"
+  proof(rule impI, rule ext)
+    fix x
+    show " abs1 M (trans1 skip s) x = trans1 (absTransfStatement M skip) (abs1 M s) x "
+      by auto
+  qed
+next
+  fix as
+  let ?S="assign as"
+  show "?P ?S"
+  proof(rule impI, rule ext)
+    fix x
+    assume b1:" absTransfStatement M (assign as) = skip" 
+    show " abs1 M (trans1 ?S s) x = trans1 (absTransfStatement M ?S) (abs1 M s) x "
+      apply(cut_tac a1 b1,case_tac "fst as=x",auto,case_tac "fst as",auto)done
+  qed
+next
+  fix as P
+  let ?S="parallel as P"
+  assume b1:"?P P"
+  show "?P ?S"
+  proof(rule impI, rule ext)
+    fix x
+    assume c1:" absTransfStatement M ?S = skip" 
+    show " abs1 M (trans1 ?S s) x = trans1 (absTransfStatement M ?S) (abs1 M s) x "
+    proof(case_tac "absTransfVar M (fst as) = dontCareVar ")
+      assume d1:"absTransfVar M (fst as) = dontCareVar"
+      show "abs1 M (trans1 (parallel as P) s) x =
+      trans1 (absTransfStatement M (parallel as P)) (abs1 M s) x"
+      
+      proof -
+        have f1: "\<And>v. abs1 M (trans1 P s) v = trans1 skip (abs1 M s) v"
+          using absTransfStatement.simps(3) b1 c1 d1 by presburger
+        obtain nn :: "varType \<Rightarrow> nat \<Rightarrow> nat" and ccs :: "varType \<Rightarrow> nat \<Rightarrow> char list" where
+          f2: "\<And>v n f na nb va cs fa fb fc fd. (v \<noteq> dontCareVar \<or> n < nn v n \<or> abs1 n f v = dontCare) \<and> (\<not> na < nb \<or> va \<noteq> Para cs nb \<or> abs1 na fa va = dontCare) \<and> (v = dontCareVar \<or> n < nn v n \<or> abs1 n fb v = absTransfConst n (fb v)) \<and> (v \<noteq> dontCareVar \<or> Para (ccs v n) (nn v n) = v \<or> abs1 n fc v = dontCare) \<and> (v = dontCareVar \<or> Para (ccs v n) (nn v n) = v \<or> abs1 n fd v = absTransfConst n (fd v))"
+          by moura
+        moreover
+        { assume "dontCareVar \<noteq> x"
+          have "fst as \<noteq> x \<and> dontCareVar \<noteq> x \<and> fst as \<noteq> x \<and> dontCareVar \<noteq> x \<or> abs1 M (trans1 (parallel as P) s) x = trans1 skip (abs1 M s) x"
+            using f2 f1 by (metis absTransfVar.simps(1) absTransfVar.simps(2) d1 varType.exhaust)
+          then have "abs1 M (trans1 (parallel as P) s) x = trans1 skip (abs1 M s) x"
+            using f2 f1 by (metis (full_types) trans1.simps(3)) }
+        ultimately show ?thesis
+          using f1 by (metis (full_types) c1)
+      qed
+    next
+      assume d1:"absTransfVar M (fst as) \<noteq> dontCareVar"
+      have False
+        using c1 d1 by auto
+      then show   ?thesis 
+        by auto
+    qed
+  qed
+qed
+*)
+   
+
+lemma stateAbs:
+   assumes a0:"s dontCareVar =dontCare" 
+   shows "(mutualDiffDefinedStmList LS \<and>
+  (\<forall>S. (S \<in>set LS) \<longrightarrow>   ((absTransfStatement M S) =skip \<or> 
+    abs1 M (trans1 S s) = trans1 (absTransfStatement M S) (abs1 M s)))) \<longrightarrow>
+    abs1 M (trans1 (parallelList LS) s) = 
+    trans1 (absTransfStatement M (parallelList LS)) (abs1 M s) " (is "?P LS")
+  sorry
+(*proof(induct_tac LS)
+  show "?P []"
+    by auto
+next
+  fix S LS
+  assume a1:"?P LS" (is "?ant1 LS \<and>?ant2 LS  \<longrightarrow>?cons LS")
+  show "?P (S#LS)" 
+  proof((rule impI)+)
+    assume b0:"?ant1 (S#LS) \<and>?ant2 (S#LS)"
+    show "?cons (S#LS)"
+    proof(case_tac "S")
+      assume b1:"S=skip"
+      have b2:"parallelList (S # LS) =parallelList LS"
+        by (simp add: b1)
+      have b3:"?ant1 LS"
+        by(cut_tac b0,auto)
+      have b3a:"?ant2 LS"
+        by(cut_tac b0,auto)
+      have b4:"?cons LS"
+        using b3 b3a local.a1 by blast
+        
+      show " abs1 M (trans1 (parallelList (S # LS)) s)  =
+         trans1 (absTransfStatement M (parallelList (S # LS))) (abs1 M s)  "
+        using b2 b4 by presburger 
+    next
+      fix as2
+      assume b1:"S=assign as2 "
+      show " abs1 M (trans1 (parallelList (S # LS)) s)  =
+         trans1 (absTransfStatement M (parallelList (S # LS))) (abs1 M s)  "
+      proof -
+      have b2:"parallelList (S # LS) =parallel as2 (parallelList LS)"
+        by (simp add: b1)
+      have b3:"?ant1 LS"
+        by(cut_tac b0,auto)
+      have b3a:"?ant2 LS"
+        by(cut_tac b0,auto)
+      have b4:"?cons LS"
+        using b3 b3a local.a1 by blast
+      have b5:" abs1 M (trans1 (parallel as2 (parallelList LS)) s)  =
+         trans1 (absTransfStatement M (parallel as2 (parallelList LS))) (abs1 M s)  "
+      proof
+        fix x
+        show "abs1 M (trans1 (parallel as2 (parallelList LS)) s) x =
+         trans1 (absTransfStatement M (parallel as2 (parallelList LS))) (abs1 M s) x"
+        proof -
+        have c0:"(fst as2\<noteq>x) \<or> ~(fst as2\<noteq>x)"
+          by auto
+
+        moreover
+        {assume c1:"fst as2\<noteq>x"
+         
+          have d1:" abs1 M (trans1 (parallel as2 (parallelList LS)) s) x =
+          trans1 (absTransfStatement M (parallel as2 (parallelList LS))) (abs1 M s) x "
+            apply(cut_tac  c1,auto)
+            apply (metis abs1_def b4)
+            apply (metis One_nat_def abs1_def add.right_neutral add_Suc_right b3 
+                  b3a local.a1)
+            by (metis abs1_def b3 b3a local.a1)
+            
+             
+        }
+
+        {assume c1:"~(fst as2\<noteq>x)"
+          have c1:"fst as2=x" by(cut_tac c1,auto)
+          have c2:"fst as2\<noteq>dontCareVar" sorry
+          have c3:"abs1 M (trans1 (parallel as2 (parallelList LS)) s) x =
+                (abs1 M ((trans1 (assign as2) s)) x)"
+            apply(cut_tac c1,auto)done 
+          have c4:"(EX v n. x=Para v n \<and> n>M) | \<not>(EX v n. x=Para v n \<and> n>M)"
+            by blast
+
+          moreover
+          {assume c4:"(EX v n. x=Para v n \<and> n>M)"
+           have c5:"abs1 M ((trans1 (assign as2) s)) x= dontCare
+                  "
+             apply(cut_tac c1 c4,auto)  done
+
+           have c6:"x \<notin>varOfSents LS" sorry
+           have c7:"x \<notin>varOfSent (absTransfStatement M (parallelList LS))" sorry
+
+           have c7:"trans1 (absTransfStatement M (parallel as2 (parallelList LS)))
+             (abs1 M s) x =dontCare" 
+              
+             apply(cut_tac c1 c4 c7,auto)
+             by (metis abs1_def b4)   
+
+           have c8:" abs1 M (trans1 (parallel as2 (parallelList LS)) s) x =
+            trans1 (absTransfStatement M (parallel as2 (parallelList LS))) (abs1 M s) x "
+             (is "?LHS =?RHS")
+             using c3 c5 c7 by auto
+          }
+          moreover
+          {assume c4:"~(EX v n. x=Para v n \<and> n>M)"
+            have "x=dontCareVar \<or> ~x=dontCareVar"
+              by blast
+            moreover
+            {assume c41:"~x=dontCareVar"
+            have c5:"abs1 M ((trans1 (assign as2) s)) x= 
+              absTransfConst M (expEval (snd as2) s)"       
+              apply(cut_tac c1 c4 c41,auto)  done 
+
+            have c7:"trans1 (absTransfStatement M (parallel as2 (parallelList LS)))
+             (abs1 M s) x = absTransfConst M (expEval (snd as2) s)" 
+              
+             apply(cut_tac c1 c2 c4 ,auto)
+             apply (metis absTransfVar.simps(1) absTransfVar.simps(2) varType.exhaust)
+              by (metis absTransfStatement.simps(2) b0 b1 c5 fst_conv list.set_intros(1)
+                  snd_conv statement.distinct(1) trans1.simps(2))
+            have c8:" abs1 M (trans1 (parallel as2 (parallelList LS)) s) x =
+            trans1 (absTransfStatement M (parallel as2 (parallelList LS))) (abs1 M s) x "
+             (is "?LHS =?RHS")
+              using c3 c5 c7 by auto 
+          }
+           moreover
+           {assume c41:"x=dontCareVar"
+             
+             have c11:" abs1 M (trans1 (parallel as2 (parallelList LS)) s) x =
+            trans1 (absTransfStatement M (parallel as2 (parallelList LS))) (abs1 M s) x "
+             (is "?LHS =?RHS")
+               using c1 c2 c41 by blast
+          }
+          ultimately have d1:"abs1 M (trans1 (parallel as2 (parallelList LS)) s) x =
+            trans1 (absTransfStatement M (parallel as2 (parallelList LS))) (abs1 M s) x"
+            by blast
+        }
+       ultimately have "abs1 M (trans1 (parallel as2 (parallelList LS)) s) x =
+            trans1 (absTransfStatement M (parallel as2 (parallelList LS))) (abs1 M s) x"
+         
+         using \<open>fst as2 \<noteq> x \<Longrightarrow>
+     abs1 M (trans1 (parallel as2 (parallelList LS)) s) x =
+     trans1 (absTransfStatement M (parallel as2 (parallelList LS))) (abs1 M s) x\<close> by blast
+     }
+    ultimately show "abs1 M (trans1 (parallel as2 (parallelList LS)) s) x =
+            trans1 (absTransfStatement M (parallel as2 (parallelList LS))) (abs1 M s) x"
+      using \<open>fst as2 \<noteq> x \<Longrightarrow> abs1 M (trans1 (parallel as2 (parallelList LS)) s) x = 
+      trans1 (absTransfStatement M (parallel as2 (parallelList LS))) (abs1 M s) x\<close> by blast
+      
+     qed
+   qed
+       show " abs1 M (trans1 (parallelList (S # LS)) s) =
+          trans1 (absTransfStatement M (parallelList (S # LS))) (abs1 M s)"
+     using b2 b5 by auto
+      qed
+    next
+      fix x31 x32
+      assume b1:"S = parallel x31 x32"
+      show " abs1 M (trans1 (parallelList (S # LS)) s)  =
+         trans1 (absTransfStatement M (parallelList (S # LS))) (abs1 M s)  "
+      proof 
+        fix x
+        show "abs1 M (trans1 (parallelList (S # LS)) s) x =
+         trans1 (absTransfStatement M (parallelList (S # LS))) (abs1 M s) x "
+        proof(case_tac "x \<in> varOfSent S")
+          assume c1:"x \<in> varOfSent S"
+           show "abs1 M (trans1 (parallelList (S # LS)) s) x =
+            trans1 (absTransfStatement M (parallelList (S # LS))) (abs1 M s) x "
+           proof -
+             have c2:"abs1 M (trans1 (parallelList (S # LS)) s) x =
+                    abs1 M (trans1 S  s) x"
+               using b0 c1 stateAbsAux1 mutualDiffDefinedStmList.simps(2) by blast
+             have c3:"trans1 (absTransfStatement M (parallelList (S # LS))) (abs1 M s) x=
+                trans1 (absTransfStatement M (  (S ))) (abs1 M s) x"
+               using b0 c1 stateAbsAux2 mutualDiffDefinedStmList.simps(2) by blast 
+             have c4:"abs1 M (trans1 S  s) x=
+                 trans1 (absTransfStatement M (  (S ))) (abs1 M s) x"
+             proof(case_tac "absTransfStatement M (  (S )) = skip ")
+               assume d1: "absTransfStatement M (  (S )) = skip"
+               show "abs1 M (trans1 S s) x = trans1 (absTransfStatement M S) (abs1 M s) x"
+                 by (simp add: absStmIsSkip assms d1) 
+             next
+               assume d1:"\<not>absTransfStatement M (  (S )) = skip"
+               show "abs1 M (trans1 S s) x = trans1 (absTransfStatement M S) (abs1 M s) x"
+                 by (meson b0 d1 list.set_intros(1)) 
+             qed
+            show "abs1 M (trans1 (parallelList (S # LS)) s) x =
+            trans1 (absTransfStatement M (parallelList (S # LS))) (abs1 M s) x "
+              using c2 c3 c4 by auto
+          qed
+        next
+          assume c1:"x \<notin> varOfSent S"
+           show "abs1 M (trans1 (parallelList (S # LS)) s) x =
+            trans1 (absTransfStatement M (parallelList (S # LS))) (abs1 M s) x "
+           proof -
+            have c2:"abs1 M (trans1 (parallelList (S # LS)) s) x =
+                    abs1 M (trans1 (parallelList ( LS))  s) x"
+            
+              using b0 c1 stateAbsAux3 mutualDiffDefinedStmList.simps(2) by blast
+
+             have c3:"trans1 (absTransfStatement M (parallelList (S # LS))) (abs1 M s) x=
+                trans1 (absTransfStatement M (parallelList  (LS ))) (abs1 M s) x"
+               using b0 c1 stateAbsAux4 mutualDiffDefinedStmList.simps(2) by blast 
+
+             have c4:"abs1 M (trans1 (parallelList ( LS))  s) x=
+                     trans1 (absTransfStatement M (parallelList  (LS ))) (abs1 M s) x "
+               by (meson b0 list.set_intros(2) local.a1 mutualDiffDefinedStmList.simps(2))
+              show "abs1 M (trans1 (parallelList (S # LS)) s) x =
+            trans1 (absTransfStatement M (parallelList (S # LS))) (abs1 M s) x "
+              using c2 c3 c4 by auto
+          qed   
+        qed
+      qed
+    qed
+  qed
+qed
+*)
+
+lemma wellDefinedForStatementIsmutualDiffDefinedStmList:
+  assumes a1:"wellDefinedForStatement s a N M f (  LS)"  
+  shows "mutualDiffDefinedStmList LS" sorry
+(*proof -
+  have a1:" LS=map f (down N) \<and> (\<forall>i. (isBoundAssign s a i M (f i)))"
+    apply(cut_tac a1,unfold wellDefinedForStatement_def,auto)
+    done
+  have "\<forall>N. (LS=map f (down N) \<and> (\<forall>i. (isBoundAssign  s a i M (f i))))
+   \<longrightarrow>mutualDiffDefinedStmList LS" (is "?P LS")
+  proof(induct_tac LS)
+    show "?P []"
+      apply(unfold isBoundAssign_def,auto)done
+    next
+      fix l L
+      assume b1:"?P L"
+      show "?P (l#L)"
+      proof(rule allI,rule impI)
+        fix N
+        assume c1:"l # L = map f (down N) \<and> (\<forall>i. isBoundAssign s a i M (f i))"
+        show "mutualDiffDefinedStmList (l # L) "
+        proof(simp)
+          have "(\<exists>N'.  N=Suc N')|N=0" apply arith done 
+          moreover
+          {assume d1:"N=0"
+            have "varOfSent l \<inter> varOfSents L = {} \<and> 
+            mutualDiffDefinedStmList L \<and> mutualDiffDefinedStm l"
+              apply(cut_tac c1 d1, auto) thm spec
+              apply(drule_tac x="0" in spec) 
+              apply(case_tac "f 0",auto)
+              done
+          }
+          moreover
+          {assume d1:"(\<exists>N'.  N=Suc N')"
+            from d1 obtain N' where d1:"N = Suc N'"
+              by blast
+            from c1 have d2:"l=f (Suc N') \<and> L=map f (down N')"
+              using d1 by auto
+            have d3:"\<exists>v. varOfSent l= { Para v (Suc N')}"
+              apply(cut_tac c1 d1 d2)
+              apply(erule conjE)
+              apply(drule_tac x="Suc N'" in spec,case_tac "f (Suc N')",auto)
+              done
+            have d4:"L=map f (down N')\<longrightarrow>
+              (\<forall>i. isBoundAssign s a i M (f i))\<longrightarrow>
+                varOfSents L = {x. \<exists> i. x=Para a i \<and> i \<le>N'}" (is "?R N'")
+            proof(induct_tac N')
+              show "?R 0"
+              proof( simp,(rule impI)+)
+                assume e1:"\<forall>i. isBoundAssign s a i M (f i) "
+                have e2:"isBoundAssign s a 0 M (f 0) "
+                  using e1 by blast
+                have e3:"\<exists>  e. (f 0) = assign ((Para a 0), e)" 
+                  apply(cut_tac e2,case_tac "f 0",auto) done
+                then obtain  e where e3:"(f 0) = assign ((Para a 0), e)" 
+                  by blast
+                show "varOfSent (f 0) = { Para a 0}"
+                  apply(cut_tac e3,simp)
+                  done
+              qed
+            next
+              fix n
+              assume b1:"?R n"
+              show "?R (Suc n)"
+                sorry
+            qed
+
+            have "varOfSent l \<inter> varOfSents L = {} \<and> 
+            mutualDiffDefinedStmList L \<and> mutualDiffDefinedStm l"
+              apply(cut_tac c1 d2, auto) thm spec
+              apply(drule_tac x="z" in spec) 
+              apply(case_tac "f z",force+)
+              using c1 d3 d4 apply auto[1]
+                apply force
+              apply (metis b1)
+              by (metis isBoundAssign.simps(3) mutualDiffDefinedStm.simps(1) mutualDiffDefinedStm.simps(2) statement.exhaust) 
+               
+          }
+          ultimately   
+          show "varOfSent l \<inter> varOfSents L = {} \<and>
+           mutualDiffDefinedStmList L \<and> mutualDiffDefinedStm l"
+            by blast
+        qed
+      qed
+    qed
+    show "mutualDiffDefinedStmList LS"
+      using \<open>\<forall>N. LS = map f (down N) \<and>
+ (\<forall>i. isBoundAssign s a i M (f i)) \<longrightarrow> mutualDiffDefinedStmList LS\<close> local.a1 by blast
+  qed
+*)
+lemma stateAbsAnother:
+   assumes a0:"s dontCareVar =dontCare" 
+   shows "(mutualDiffDefinedStm LS ) \<longrightarrow>
+    abs1 M (trans1 ( LS) s) = 
+    trans1 (absTransfStatement M ( LS)) (abs1 M s) " (is "?P LS")
+  sorry
+(*lemma statementSim:
+  assumes a1:"wellFormedParallel s i M N S"  
+  shows "abs1 M (trans1 S s) = trans1 (absTransfStatement M S) s"*)
+
+lemma topAbsSafeExpForm:
+   
+  shows "(safeExp s i M e \<longrightarrow>i>M \<longrightarrow>((topTransfExp (absTransfExp  M e))=dontCareExp  \<or>
+   (topTransfExp (absTransfExp  M e))   =(absTransfExp  M e))) \<and>
+  (safeFormula s i M f  \<longrightarrow>i>M\<longrightarrow>(((topTransfForm (absTransfForm  M f)=chaos ) \<or>
+  ((absTransfForm  M f) =  (topTransfForm (absTransfForm  M f))  ))))"
+   (is "?Pe e s \<and>   ?Pf f s") 
+  sorry
+
+lemma wellForallForm1:
+  assumes a1:"safeFormula s i M g " and a2:"formEval    ( (forallForm fg N)) s "
+  shows "  formEval  ( topTransfForm (absTransfForm M (forallForm fg N))) s"
+  sorry
+
+
+(*theorem protSimLemma:
+  assumes 
+protSim I I1 rs rs1 M*)
+(*inductive_set simpleFormedExpSet :: "nat \<Rightarrow> expType set" and
+simpleFormedFormulaSet::"nat\<Rightarrow>formula set" 
+  for i::"nat"  where
+
+  simpleGlobalVarExp: "IVar ((Ident) x )\<in> simpleFormedExpSet i" |
+
+  simplelocalVarExp: "IVar (Para n i)  \<in> simpleFormedExpSet i" |
+
+  simpleIteExp: "\<lbrakk>e1 \<in> simpleFormedExpSet i;e2 \<in> simpleFormedExpSet i;
+             f \<in> simpleFormedFormula i\<rbrakk> \<Longrightarrow>
+             iteForm f e1 e2 \<in> simpleFormedExpSet i" |
+
+  simpleChaosForm: "chaos \<in> simpleFormedFormulaSet i"|
+
+  simpleMiracleForm:"miracle \<in> simpleFormedExpSet i"|
+  simpleEqnForm:" \<lbrakk>e1 \<in> simpleFormedExpSet i;e2 \<in> simpleFormedExpSet i\<rbrakk>\<Longrightarrow>
+          eqn e1 e2  \<in> simpleFormedFormulaSet i"|
+
+  simpleNegForm:" \<lbrakk>f1 \<in> simpleFormedFormulaSet i \<rbrakk>\<Longrightarrow>
+          neg f1  \<in> simpleFormedFormulaSet i" | 
+
+  simpleAndForm:" \<lbrakk>f1 \<in> simpleFormedFormulaSet i; f2 \<in> simpleFormedFormulaSet i \<rbrakk>\<Longrightarrow>
+          andForm f1 f2 \<in> simpleFormedFormulaSet i" |
+
+  simpleOrForm:" \<lbrakk>f1 \<in> simpleFormedFormulaSet i; f2 \<in> simpleFormedFormulaSet i \<rbrakk>\<Longrightarrow>
+          orForm f1 f2 \<in> simpleFormedFormulaSet i"|
+
+  simpleImplyForm:" \<lbrakk>f1 \<in> simpleFormedFormulaSet i; f2 \<in> simpleFormedFormulaSet i \<rbrakk>\<Longrightarrow>
+          implyForm f1 f2 \<in> simpleFormedFormulaSet i"
+
+definition wellFormedAndList1::"nat \<Rightarrow> formula \<Rightarrow>bool " where
+"wellFormedAndList1  N f\<equiv> (\<exists>N fg. f=andList (map (\<lambda>i. fg i) (down N)) \<and>
+( \<forall>i. (fg i)\<in> (simpleFormedFormulaSet i)))"
+
+definition wellFormedAndList2::"nat \<Rightarrow> nat\<Rightarrow>formula \<Rightarrow>bool " where
+"wellFormedAndList2  N i f\<equiv> (\<exists>N fg. f=
+  andList (map (\<lambda>j. implyForm (neg (eqn (Const (index i)) (Const (index j)))) (fg j)) (down N)) \<and>
+( \<forall>i. (fg i)\<in> (simpleFormedFormulaSet i)))"
+
+definition  wellForm::"nat \<Rightarrow> nat\<Rightarrow>formula \<Rightarrow>bool" where
+"wellForm N i f \<equiv> \<exists> fs. f=andList fs \<and> 
+  (\<forall>f. f \<in> set fs \<longrightarrow>
+  ((wellFormedAndList1  N f) \<or> (wellFormedAndList2  N i f) \<or>  (f \<in> simpleFormedFormulaSet i)))"
+
+definition wellFormedIteExp::"nat \<Rightarrow>expType \<Rightarrow> bool" where
+"wellFormedIteExp i  e\<equiv> \<exists> e1 e2 f. (e=iteForm f e1 e2) 
+  \<and> e1 \<in> simpleFormedExpSet i \<and> e2 \<in> simpleFormedExpSet i"*)
+(*(neg (eqn (Const (index i)) (Const (index j))))*)
+(*
+definition simpleAssignment::"nat \<Rightarrow> statement \<Rightarrow>bool" where
+"simpleAssignment i as \<equiv>
+\<exists> v e.  (IVar v \<in>simpleFormedExpSet i)
+ \<and>(e \<in>simpleFormedExpSet i) \<and>as= assign (v, e)"
+
+definition wellAssignment::"nat\<Rightarrow>statement \<Rightarrow>bool" where
+"wellAssignment j  as \<equiv>
+\<exists> v e.  (IVar v \<in>simpleFormedExpSet j)
+ \<and>(wellFormedIteExp  j e) \<and>as= assign (v, e)"
+
+definition wellFormedParallelStatement::"nat \<Rightarrow> nat \<Rightarrow> statement \<Rightarrow>bool" where
+"wellFormedParallelStatement N i S \<equiv>\<exists> ps.  (S=parallelList (map ps (down N) ) 
+\<and>((\<forall>i. simpleAssignment i (ps i) )| (\<forall>j. wellAssignment  j (ps j)) ))"
+*)
+(*inductive_set reachableSet :: "formula set \<Rightarrow> rule set \<Rightarrow> state set" 
+  for inis::"formula set" and rules::"rule set" where
+
+  initState: "\<lbrakk>formEval ini s; ini \<in> inis\<rbrakk> \<Longrightarrow> s \<in> reachableSet inis rules" |
+
+  oneStep: "\<lbrakk>s \<in> reachableSet inis rules;
+             r \<in> rules;
+             formEval (pre r) s\<rbrakk> \<Longrightarrow>
+             trans (act r) s \<in> reachableSet inis rules"*)
+(*
+lemma absExpForm:
+  assumes a:"s dontCareVar =dontCare" and a2:"
+  e \<in>simpleFormedExpSet i" and a3:"f \<in>simpleFormedFormulaSet i"
+  shows "((absTransfExp  M e\<noteq>dontCareExp\<longrightarrow>
+  expEval (absTransfExp  M e) (abs1 M s)  =absTransfConst M (expEval e s))) \<and>
+  ((absTransfForm  M f\<noteq>dontCareForm \<longrightarrow>formEval f s 
+\<longrightarrow>formEval (absTransfForm  M f) (abs1 M s)))"
+   (is "?Pe e s \<and>   ?Pf f s")
+  using a2 and a3
+proof(induct )
+
+  fix x
+  show "?Pe (IVar (Ident x)) s"
+  proof(case_tac "EX n. (  (s (Ident x))=(index n) )\<and> n>M")
+      assume b1:"\<exists>n.  (s (Ident x)) = index n \<and> M < n "
+      show "?Pe (IVar (Ident x)) s"
+        by(cut_tac b1 ,auto)
+    next
+      assume b1:"\<not>(\<exists>n.  (s (Ident x)) = index n \<and> M < n )"
+      show "?Pe (IVar (Ident x)) s"
+      proof(cut_tac  b1, case_tac "(s (Ident x))",auto)qed
+  qed
+    by auto
+  show "?Pe (IVar x) s"
+  proof(case_tac x) 
+    fix x1
+    assume a1:"x=Ident x1"
+    show "?Pe (IVar x) s"
+    proof(case_tac "EX n. (  (s x)=(index n) )\<and> n>M")
+      assume b1:"\<exists>n.  (s x) = index n \<and> M < n "
+      show "?Pe (IVar x) s"
+        by(cut_tac b1 a1,auto)
+    next
+      assume b1:"\<not>(\<exists>n.  (s x) = index n \<and> M < n )"
+      show "?Pe (IVar x) s"
+      proof(cut_tac a1 b1, case_tac "(s x)",auto)qed
+    qed
+  next
+    fix x21 x22
+    assume a1:"x = Para x21 x22"
+    show "?Pe (IVar x) s"
+    proof(case_tac "x22 >M")
+      assume b1:"x22>M "
+      show "?Pe (IVar x) s"
+        by(cut_tac a b1 a1,simp)
+    next
+      assume b1:"~x22>M "
+      show "?Pe (IVar x) s"
+      proof(case_tac "EX n. (  (s x)=(index n) )\<and> n>M",cut_tac a b1 a1,force)
+        assume c1:"\<nexists>n. s x = index n \<and> M < n"
+        have c2:" expEval (absTransfExp M (IVar x)) (abs1 M s) =s (Para x21 x22)"
+        proof(cut_tac a b1 a1 c1,force)qed
+        have c3:"absTransfConst M (expEval (IVar x) s)=s (Para x21 x22)"
+          apply(cut_tac a b1 a1 c1,case_tac "s x",auto) done
+        show "?Pe (IVar x) s"
+          using c2 c3 by presburger
+      qed
+    qed
+  next
+    assume a1:"x=dontCareVar"
+    show "?Pe (IVar x) s"
+      by (simp add: a1)
+
+  qed
+next
+  fix x
+  show "?Pe (Const x) s"
+  proof(case_tac x,auto)qed
+next
+  fix b e1 e2
+  assume a1:"?Pe e1 s" and a2:"?Pe e2 s"
+  and a3:"?Pf b s"
+  show "?Pe (iteForm b e1 e2) s"
+  proof(cut_tac a1 a2 a3,case_tac "((absTransfForm M b) \<noteq> dontCareForm 
+  \<and>(absTransfExp M e1) \<noteq> dontCareExp \<and>
+  (absTransfExp M e2) \<noteq> dontCareExp)",auto)
+  qed
+next
+  show "?Pe (dontCareExp) s"
+    by auto
+next
+  fix e1 e2
+  assume  a1:"?Pe e1 s" and a2:"?Pe e2 s"
+  show "?Pf (eqn e1 e2) s"
+  proof(cut_tac a1 a2 ,case_tac "( 
+  (absTransfExp M e1) = dontCareExp \<or>
+  (absTransfExp M e2) = dontCareExp)",auto)
+
+(*
+inductive isBoolVal::"state \<Rightarrow> expType \<Rightarrow> bool" where
+"s(v) =boolV b\<Longrightarrow>isBoolVal s (IVar v) " | 
+"  c =(boolV b) \<Longrightarrow>isBoolVal s (Const c)" | 
+"
+  ( (isBoolVal s e1)\<and> (isBoolVal s e2)) \<Longrightarrow>isBoolVal s (iteForm f e1 e2)   "|
+"s(v) =(enum tn vn) \<Longrightarrow>\<not>isBoolVal s (IVar v) "
+
+inductive isEnumVal::"state \<Rightarrow> expType \<Rightarrow> bool" where
+"s(v) =(enum tn vn) \<Longrightarrow>isEnumVal s (IVar v) " | 
+" c =(enum tn vn) \<Longrightarrow> isEnumVal s (Const c)  " | 
+"
+  ( (isEnumVal s e1) \<and> (isEnumVal s e2)) \<Longrightarrow>isEnumVal s (iteForm f e1 e2) "
+
+inductive isIndexVal::"state \<Rightarrow> expType \<Rightarrow> bool" where
+"s(v) =(index vn) \<Longrightarrow>isIndexVal s (IVar v) " | 
+" c =(index vn) \<Longrightarrow> isIndexVal s (Const c)  " | 
+
+"
+  ( (isIndexVal s e1) \<and> (isIndexVal s e2)) \<Longrightarrow>isIndexVal s (iteForm f e1 e2) "
+
+primrec isBoolVal::"state \<Rightarrow> expType \<Rightarrow> bool" where
+"isBoolVal s (IVar v) = (if (\<exists>b. s(v) =(boolV b)) then True else False)" | 
+"isBoolVal s (Const c) = (if (\<exists>b. c =(boolV b)) then True else False)" | 
+"isBoolVal s (iteForm f e1 e2) = 
+  ( (isBoolVal s e1)\<and> (isBoolVal s e2))"
+
+primrec isEnumVal::"state \<Rightarrow> expType \<Rightarrow> bool" where
+"isEnumVal s (IVar v) = (if (\<exists>tn vn. s(v) =(enum tn vn)) then True else False)" | 
+"isEnumVal s (Const c) = (if (\<exists>tn vn. c =(enum tn vn)) then True else False)" | 
+"isEnumVal s (iteForm f e1 e2) = 
+  ( (isEnumVal s e1) \<and> (isEnumVal s e2))"
+
+primrec isIndexVal::"state \<Rightarrow> expType \<Rightarrow> bool" where
+"isIndexVal s (IVar v) = (if (\<exists> vn. s(v) =(index vn)) then True else False)" | 
+"isIndexVal s (Const c) = (if (\<exists> vn. c =(index vn)) then True else False)" | 
+"isIndexVal s (iteForm f e1 e2) = 
+  ( (isIndexVal s e1) \<and> (isIndexVal s e2))"*)
+*)
